

# Chapter 5.1: The Derivative

## 1. Definition of the Derivative

**Historical Context:** Formulated rigorously by Cauchy (1821) using limits, moving away from vague notions of tangent lines and velocity.

### Definition 5.1.1 (The Derivative)

Let  $I \subset \mathbb{R}$  be an interval and  $f : I \rightarrow \mathbb{R}$ . For a fixed  $p \in I$ , the derivative  $f'(p)$  is:

$$f'(p) = \lim_{x \rightarrow p} \frac{f(x) - f(p)}{x - p}$$

Alternatively, letting  $x = p + h$ :

$$f'(p) = \lim_{h \rightarrow 0} \frac{f(p + h) - f(p)}{h}$$

- **Geometric interpretation:** Slope of the tangent line at  $(p, f(p))$ .
- **Physical interpretation:** Instantaneous velocity.

## 2. One-Sided Derivatives

If  $p$  is an endpoint or we need to analyze corner points, we use one-sided limits (Definition 5.1.2).

- **Right Derivative ( $f'_+(p)$ ):**  $\lim_{h \rightarrow 0^+} \frac{f(p + h) - f(p)}{h}$
- **Left Derivative ( $f'_-(p)$ ):**  $\lim_{h \rightarrow 0^-} \frac{f(p + h) - f(p)}{h}$

### Key Property:

For an interior point  $p \in I$ ,  $f'(p)$  exists **if and only if** both  $f'_+(p)$  and  $f'_-(p)$  exist and are **equal**.

## 3. Worked Examples (Specific Functions)

The text analyzes the differentiability of several specific functions to illustrate the definition.

**A. Power Function ( $f(x) = x^2$ )**

$$f'(x) = \lim_{h \rightarrow 0} \frac{(x+h)^2 - x^2}{h} = \lim_{h \rightarrow 0} (2x + h) = 2x$$

(Note: Generalizes to  $f(x) = x^n \implies f'(x) = nx^{n-1}$ ).

**B. Square Root ( $f(x) = \sqrt{x}, x > 0$ )**

Uses rationalization:

$$\frac{\sqrt{x+h} - \sqrt{x}}{h} = \frac{1}{\sqrt{x+h} + \sqrt{x}} \xrightarrow{h \rightarrow 0} \frac{1}{2\sqrt{x}}$$

**C. Sine Function ( $f(x) = \sin x$ )**

Uses the identity  $\sin(x+h) = \sin x \cos h + \cos x \sin h$ :

$$\frac{\sin(x+h) - \sin x}{h} = \sin x \left( \frac{\cos h - 1}{h} \right) + \cos x \left( \frac{\sin h}{h} \right)$$

Since  $\lim_{h \rightarrow 0} \frac{\sin h}{h} = 1$  and  $\lim_{h \rightarrow 0} \frac{\cos h - 1}{h} = 0$ ,  $f'(x) = \cos x$ .

**D. Absolute Value ( $f(x) = |x|$ ) at  $x = 0$** 

- $f'_+(0) = \lim_{h \rightarrow 0^+} \frac{h}{h} = 1$
- $f'_-(0) = \lim_{h \rightarrow 0^-} \frac{-h}{h} = -1$
- **Result:**  $f'_+(0) \neq f'_-(0)$ , so  $f$  is **not differentiable** at 0.

**E. Cusp ( $g(x) = x^{3/2}$ ) at  $x = 0$** 

$$g'(0) = \lim_{h \rightarrow 0^+} \frac{h^{3/2}}{h} = \lim_{h \rightarrow 0^+} \sqrt{h} = 0$$

Differentiable at 0.

**F. Oscillating Discontinuity ( $f(x) = x \sin(1/x)$  for  $x \neq 0$ ,  $f(0) = 0$ )**

$$f'(0) = \lim_{h \rightarrow 0} \frac{h \sin(1/h) - 0}{h} = \lim_{h \rightarrow 0} \sin\left(\frac{1}{h}\right)$$

**Result:** Limit does not exist. Not differentiable at 0.

## G. Differentiable with Discontinuous Derivative ( $g(x) = x^2 \sin(1/x)$ for $x \neq 0$ , $g(0) = 0$ )

- At  $x = 0$ :

$$g'(0) = \lim_{h \rightarrow 0} \frac{h^2 \sin(1/h)}{h} = \lim_{h \rightarrow 0} h \sin\left(\frac{1}{h}\right) = 0$$

(By Squeeze Theorem).

- For  $x \neq 0$ :  $g'(x) = 2x \sin(1/x) - \cos(1/x)$ .
- **Observation:**  $\lim_{x \rightarrow 0} g'(x)$  does not exist (due to  $\cos(1/x)$ ).
- **Conclusion:**  $g$  is differentiable everywhere, but  $g'$  is **not continuous** at 0.

## 4. Relationship between Differentiability and Continuity

### Theorem 5.1.4:

If  $f$  is differentiable at  $p$ , then  $f$  is continuous at  $p$ .

### Proof Sketch:

$$\lim_{t \rightarrow p} (f(t) - f(p)) = \lim_{t \rightarrow p} \left[ \frac{f(t) - f(p)}{t - p} \cdot (t - p) \right] = f'(p) \cdot 0 = 0$$

Thus  $\lim_{t \rightarrow p} f(t) = f(p)$ .

- **Converse:** False. Continuity does **not** imply differentiability (e.g.,  $f(x) = |x|$ ).
- **Weierstrass Function:** An example of a function continuous everywhere but differentiable nowhere.

## 5. Arithmetic of Derivatives

### Theorem 5.1.5 (Algebraic Rules)

Let  $f, g$  be differentiable at  $x$ .

### A. Sum Rule

$$(f + g)'(x) = f'(x) + g'(x)$$

## B. Product Rule

$$(fg)'(x) = f'(x)g(x) + f(x)g'(x)$$

### Key Proof Idea: The "Add and Subtract" Trick

Direct substitution creates a mixed term  $f(x+h)g(x+h)$  that cannot be factored. To fix this, we insert a "middle term" into the numerator.

### Proof Sketch:

1. **Setup:** Start with the difference quotient:

$$\frac{f(x+h)g(x+h) - f(x)g(x)}{h}$$

2. **The Trick:** Add and subtract  $f(x+h)g(x)$ :

$$\frac{f(x+h)g(x+h) - \mathbf{f(x+h)g(x)} + \mathbf{f(x+h)g(x)} - f(x)g(x)}{h}$$

3. **Group & Limit:** Separate into two parts:

$$f(x+h) \underbrace{\left[ \frac{g(x+h) - g(x)}{h} \right]}_{\rightarrow g'(x)} + g(x) \underbrace{\left[ \frac{f(x+h) - f(x)}{h} \right]}_{\rightarrow f'(x)}$$

*Note:  $f(x+h) \rightarrow f(x)$  because differentiability implies continuity.*

## C. Quotient Rule (Reciprocal Case)

To prove the quotient rule, we first focus on the derivative of the reciprocal.

### The Reciprocal Rule:

$$\left( \frac{1}{g} \right)'(x) = -\frac{g'(x)}{[g(x)]^2}$$

### Proof Sketch:

1. **Common Denominator:**

$$\frac{\frac{1}{g(x+h)} - \frac{1}{g(x)}}{h} = \frac{g(x) - g(x+h)}{h \cdot g(x+h)g(x)}$$

## 2. Extract Derivative Definition:

Recognize that  $g(x) - g(x+h) = -[g(x+h) - g(x)]$ :

$$-\underbrace{\left[ \frac{g(x+h) - g(x)}{h} \right]}_{\rightarrow g'(x)} \cdot \frac{1}{g(x+h)g(x)}$$

## 3. Take Limit ( $h \rightarrow 0$ ):

Since  $g$  is continuous,  $g(x+h) \rightarrow g(x)$ , giving the denominator  $[g(x)]^2$ .

(Note: The full Quotient Rule is simply the Product Rule applied to  $f(x) \cdot [1/g(x)]$ .)

# 6. The Chain Rule

## Theorem 5.1.6 (Composition)

If  $f$  is differentiable at  $x$  and  $g$  is differentiable at  $y = f(x)$ , then  $h = g \circ f$  is differentiable at  $x$ :

$$h'(x) = g'(f(x)) \cdot f'(x)$$

**Proof:** Linear Approximation (to avoid division by zero).

Standard limits fail if  $f(t) - f(x) = 0$ . Instead, use "error terms" ( $u, v$ ) that go to 0:

- $f: f(t) - f(x) = (t - x)[f'(x) + u(t)]$
- $g: g(s) - g(y) = (s - y)[g'(y) + v(s)]$
- Set  $s = f(t)$  and  $y = f(x)$ . The difference quotient becomes:

$$\frac{g(f(t)) - g(f(x))}{t - x} = [f'(x) + u(t)] \cdot [g'(y) + v(f(t))]$$

- As  $t \rightarrow x$ , the error terms vanish ( $u, v \rightarrow 0$ ), leaving  $f'(x)g'(y)$ .

## Examples:

- **Composite Trig:**  $h(x) = \sin(1/x^2)$ .

$$h'(x) = \cos\left(\frac{1}{x^2}\right) \cdot \frac{d}{dx}(x^{-2}) = \cos\left(\frac{1}{x^2}\right) \cdot (-2x^{-3})$$

- **Power Rule Extension:**  $\frac{d}{dx}[f(x)]^n = n[f(x)]^{n-1}f'(x)$ .